theories/memory.v
@@ -11,17 +11,21 @@ Unset Printing Implicit Defensive.
 
 Section Memory.
 
+  (* Some constants regarding Wasm memory *)
+  Definition page_size : N := 65536%N.
+
+  Definition page_limit : N := 65536%N.
+
+  Definition byte_limit : N := N.mul page_size page_limit.
+
   Class Memory := {
       mem_t : Type;
       mem_make : byte -> N -> mem_t;
       mem_length : mem_t -> N;
       mem_lookup : N -> mem_t -> option byte;
-      mem_grow : N -> mem_t -> mem_t;
+      (* Doesn't have to succeed *)
+      mem_grow : N -> mem_t -> option mem_t;
       mem_update : N -> byte -> mem_t -> option mem_t;
-
-      mem_eq_dec:
-      forall (m1 m2: mem_t),
-        {m1 = m2} + {m1 <> m2};
       
       mem_lookup_oob :
       forall mem i,
@@ -30,18 +34,13 @@ Section Memory.
       
       mem_make_length :
       forall b len,
-        mem_length (mem_make b len) = len;
+        mem_length (mem_make b len) = N.min len byte_limit;
 
       mem_make_lookup :
       forall i len b,
-        N.lt i len ->
+        N.lt i (N.min len byte_limit) ->
         mem_lookup i (mem_make b len) = Some b;
       
-(*      mem_update_exists :
-      forall mem i b,
-        N.lt i (mem_length mem) ->
-        { mem' | mem_update i b mem = Some mem'};*)
-
       mem_update_lookup :
       forall mem mem' i b,
         mem_update i b mem = Some mem' ->
@@ -61,26 +60,15 @@ Section Memory.
       mem_grow_lookup :
       forall i n mem mem',
         N.lt i (mem_length mem) ->
-        mem_grow n mem = mem' ->
+        mem_grow n mem = Some mem' ->
         mem_lookup i mem' = mem_lookup i mem;
 
       mem_grow_length :
       forall n mem mem',
-        mem_grow n mem = mem' ->
+        mem_grow n mem = Some mem' ->
         mem_length mem' = N.add (mem_length mem) n;
     }.
 
 Context `{Memory}.
   
-Definition mem_eqb v1 v2 : bool := mem_eq_dec v1 v2.
-Definition eqmemP : Equality.axiom mem_eqb :=
-  eq_dec_Equality_axiom mem_eq_dec.
-
-HB.instance Definition mem_eqMixin := hasDecEq.Build mem_t eqmemP.
-  
 End Memory.
-
-(* Some constants regarding Wasm memory *)
-Definition page_size : N := 65536%N.
-
-Definition page_limit : N := 65536%N.
