theories/memory_vec.v
@@ -17,7 +17,9 @@ Unset Printing Implicit Defensive.
 Open Scope N_scope.
 
 (* Persistent vector, but removing some functions and relaxing the max_length
-   to 2^32-1. *)
+   to 2^32-1. Also adding a different method of creating an array for
+   growing vectors.
+ *)
 Section Array.
 
 Context {A: Type}.
@@ -29,14 +31,14 @@ Parameter arr_make : PrimInt63.int -> A -> array A.
    Does not overflow if the length exceeds the make length.
    This is used in the vector_grow function.
  *)
-Parameter arr_make_init: PrimInt63.int -> A -> array A -> PrimInt63.int -> array A.
+Parameter arr_make_copy: PrimInt63.int -> A -> array A -> PrimInt63.int -> array A.
 Parameter arr_get : array A -> PrimInt63.int -> A.
 Parameter arr_default : array A -> A.
 Parameter arr_set : array A -> PrimInt63.int -> A -> array A.
 Parameter arr_length : array A -> PrimInt63.int.
 Parameter arr_copy : array A -> array A.
 
-Definition max_arr_length : PrimInt63.int := Uint63.of_Z (Zpos 0xffffffff).
+Definition max_arr_length : PrimInt63.int := Uint63.of_Z (Z.of_N byte_limit).
 
 Notation " t .[ i ] " := (arr_get t i) (at level 5).
 Notation " t .[ i <- a ] " := (arr_set t i a) (at level 5).
@@ -56,29 +58,29 @@ Parameter default_set :
 Parameter get_make :
   forall (a : A) (size i : PrimInt63.int),
     (arr_make size a).[i] = a.
-Parameter get_make_init:
+Parameter get_make_copy:
   forall (a: A) (size i: PrimInt63.int) (t: array A) (initlen: PrimInt63.int),
     PrimInt63.ltb i size ->
     PrimInt63.leb initlen (arr_length t) ->
     PrimInt63.ltb i (arr_length t) ->
-    (arr_make_init size a t initlen).[i] = t.[i].
-Parameter get_make_init_default:
+    (arr_make_copy size a t initlen).[i] = t.[i].
+Parameter get_make_copy_default:
   forall (a: A) (size i: PrimInt63.int) (t: array A) (initlen: PrimInt63.int),
     PrimInt63.ltb i size ->
     PrimInt63.leb initlen (arr_length t) ->
     PrimInt63.leb initlen i ->
-    (arr_make_init size a t initlen).[i] = a.
+    (arr_make_copy size a t initlen).[i] = a.
 Parameter leb_length :
   forall (t : array A),
     PrimInt63.leb (arr_length t) max_arr_length = true.
 Parameter length_make :
   forall (size : PrimInt63.int) (a : A),
     arr_length (arr_make size a) =
-      (if PrimInt63.leb size max_arr_length then size else max_arr_length).
-Parameter length_make_init :
+      Uint63.min size max_arr_length.
+Parameter length_make_copy :
   forall (size : PrimInt63.int) (a : A) (t: array A) (initlen: PrimInt63.int),
-    arr_length (arr_make_init size a t initlen) =
-      (if PrimInt63.leb size max_arr_length then size else max_arr_length).
+    arr_length (arr_make_copy size a t initlen) =
+      Uint63.min size max_arr_length.
 Parameter length_set :
   forall (t : array A) (i : PrimInt63.int) (a : A),
     arr_length t.[i<-a] = arr_length t.
@@ -125,62 +127,108 @@ Section vector.
       v_size: N;
       v_capacity: N;
       v_init: T;
-      (*v_size_valid: v_size <= v_capacity;
-      v_capacity_eq: v_capacity = Uint63_to_N (arr_length v_data);*)
+      v_size_valid: v_size <= v_capacity;
+      v_capacity_eq: v_capacity = Uint63_to_N (arr_length v_data);
     }.
 
-  Coercion Uint63.of_Z: Z >-> PrimInt63.int.
-
-  Coercion Uint63_of_N: N >-> PrimInt63.int.
-
-  Coercion Uint63_of_positive: positive >-> PrimInt63.int.
-
-  Definition vector_len vec : N :=
+  Definition vector_length vec : N :=
     vec.(v_size).
 
-  Definition vector_make (len: N) x : vector :=
-    Build_vector (arr_make len x) len len x.
-
+  Definition vector_make (len: N) x : vector.
+  Proof.
+    remember (N.min len byte_limit) as capped_len.
+    refine (@Build_vector (arr_make (Uint63_of_N capped_len) x) capped_len capped_len x _ _).
+    - by lias.
+    - rewrite length_make; subst.
+      unfold max_arr_length, Uint63_to_N, Uint63_of_N.
+      rewrite Uint63.min_spec Znat.Z2N.inj_min.
+      repeat rewrite of_Z_spec.
+      repeat rewrite Znat.Z2N.inj_mod => //; try by lias.
+      repeat rewrite Znat.N2Z.id.
+      rewrite N.mod_small; cbn; by lias.
+  Defined.
+    
   Definition vector_lookup vec n : option T :=
-    if n <? vector_len vec then
-      Some (arr_get vec.(v_data) n)
+    if n <? vector_length vec then
+      Some (arr_get vec.(v_data) (Uint63_of_N n))
     else None.
 
-  Definition vector_update vec n x : option vector :=
-    if n <? vector_len vec then
-      Some (Build_vector (arr_set vec.(v_data) n x) vec.(v_size) vec.(v_capacity) vec.(v_init))
-    else None.
-          
-  Definition vector_grow vec n : vector :=
-    let newsize := vector_len vec + n in
-    if newsize <=? vec.(v_capacity) then
-      Build_vector vec.(v_data) newsize vec.(v_capacity) vec.(v_init)
-    else
-      let new_capacity := N.max newsize (vec.(v_capacity) * 2%N) in
-      let x := vec.(v_init) in
-      let new_vd := arr_make_init new_capacity x vec.(v_data) vec.(v_size) in
-      Build_vector new_vd newsize new_capacity x.
-  
+  Definition vector_update (vec: vector) (n: N) (x: T) : option vector.
+  Proof.
+    refine
+    (if n <? vector_length vec then
+      Some (@Build_vector (arr_set vec.(v_data) (Uint63_of_N n) x) vec.(v_size) vec.(v_capacity) vec.(v_init) _ _)
+     else None).
+    - by apply v_size_valid.
+    - rewrite length_set.
+      by apply v_capacity_eq.
+  Defined.
+
+  Lemma N_min_idem_r : forall n m,
+      N.min (N.min n m) m = N.min n m.
+  Proof.
+    by lias.
+  Qed.
+
+  Program Definition vector_grow (vec: vector) (n: N) : option vector :=
+    let newsize := vector_length vec + n in
+    match newsize <=? byte_limit as p1 return ((newsize <=? byte_limit) = p1) -> _ with
+    | true => (fun _ => 
+        match newsize <=? vec.(v_capacity) as p2 return (newsize <=? vec.(v_capacity) = p2) -> _ with
+        | true =>
+            (fun _ => Some (@Build_vector vec.(v_data) newsize vec.(v_capacity) vec.(v_init) _ _))
+        | false =>
+            let new_capacity := (N.min (N.max newsize (vec.(v_capacity) * 2%N)) byte_limit) in
+            let x := vec.(v_init) in
+            let new_vd := arr_make_copy (Uint63_of_N new_capacity) x vec.(v_data) (Uint63_of_N vec.(v_size)) in
+            (fun _ => Some (@Build_vector new_vd newsize new_capacity x _ _))
+        end (Logic.eq_refl (newsize <=? vec.(v_capacity))))
+    | false => (fun _ => None)
+    end (Logic.eq_refl (newsize <=? byte_limit)).
+  Next Obligation.
+    by lias.
+  Qed.
+  Next Obligation.
+    by apply v_capacity_eq.
+  Qed.
+  Next Obligation.
+    move/N.leb_spec0 in e0.
+    by lias.
+  Qed.
+  Next Obligation.
+    rewrite length_make_copy.
+    unfold Uint63_to_N, Uint63_of_N.
+    rewrite min_spec Znat.Z2N.inj_min of_Z_spec.
+    rewrite Znat.Z2N.inj_mod; try by lias.
+    rewrite Znat.N2Z.id.
+    rewrite N.mod_small; cbn; by lias.
+  Qed.
+
+  Lemma vector_size_bound: forall vec,
+      v_size vec <= byte_limit.
+  Proof.
+    move => vec.
+    specialize (@v_size_valid vec) as Hvalid.
+    specialize (v_capacity_eq vec) as Hcap.
+    unfold Uint63_to_N in Hcap.
+    rewrite Hcap in Hvalid.
+    specialize (leb_length (v_data vec)) as Hlenub; move/Uint63.lebP in Hlenub.
+    unfold max_arr_length in Hlenub.
+    clear Hcap.
+    cbn in *; by lias.
+  Qed.
+
 End vector.
 
 Section MemoryVec.
 
   Definition memory_vec : Type := @vector byte.
-  Definition mv_length := @vector_len byte.
+  Definition mv_length := @vector_length byte.
   Definition mv_make n b := @vector_make byte b n.
   Definition mv_lookup i v := @vector_lookup byte v i.
   Definition mv_update i b v:= @vector_update byte v i b.
   Definition mv_grow n v:= @vector_grow byte v n.
 
-Axiom array_neq: forall (mem1 mem2: memory_vec),
-    mem1 <> mem2.
-
-  Lemma mv_eq_dec: forall (mem1 mem2: memory_vec),
-      {mem1 = mem2} + {mem1 <> mem2}.
-  Proof.
-    right; apply array_neq.
-  Qed.
-  
   Lemma mv_lookup_oob:
     forall mem i,
       (i >= mv_length mem)%N ->
@@ -196,14 +244,14 @@ Axiom array_neq: forall (mem1 mem2: memory_vec),
   Qed.
 
   Lemma mv_make_length:
-    forall b len, mv_length (mv_make b len) = len.
+    forall b len, mv_length (mv_make b len) = N.min len byte_limit.
   Proof.
     done.
   Qed.
     
   Lemma mv_make_lookup:
     forall i len b,
-      (i < len)%N ->
+      (i < N.min len byte_limit) ->
       mv_lookup i (mv_make b len) = Some b.
   Proof.
     move => i len b Hlen /=.
@@ -236,10 +284,24 @@ Qed.
     remove_bools_options => /=.
     rewrite Hif.
     rewrite get_set_same => //.
-    unfold vector_len in Hif.
-    apply/Uint63.ltbP.
-    admit.
-  Admitted.
+    unfold vector_length in Hif.
+    specialize (v_capacity_eq mem) as Hcap.
+    specialize (@v_size_valid _ mem) as Hsize.
+    move/N.ltb_spec0 in Hif.
+    apply/ltbP.
+    unfold Uint63_of_N.
+    unfold Uint63_to_N in Hcap.
+    rewrite of_Z_spec.
+    apply (f_equal Z.of_N) in Hcap.
+    rewrite Znat.Z2N.id in Hcap.
+    - rewrite - Hcap.
+      assert (Z.of_N i mod wB <= Z.of_N i)%Z as Hbound.
+      { apply Z.mod_le; by lias. }
+      (* lots of transitivity *)
+      by lias.
+    - specialize (to_Z_bounded (arr_length (v_data mem))).
+      by lias.
+  Qed.
 
 Lemma mv_update_lookup_ne:
   forall mem mem' i j b,
@@ -248,37 +310,92 @@ Lemma mv_update_lookup_ne:
     mv_lookup i mem' = mv_lookup i mem.
 Proof.
   move => mem mem' i j b Hneq Hupdate.
-  unfold mv_lookup.
-  admit.
-Admitted.
+  unfold mv_lookup, vector_lookup.
+  unfold mv_update, vector_update in Hupdate.
+  remove_bools_options => /=.
+  move/N.ltb_spec0 in Hif.
+  unfold vector_length.
+  destruct (i <? v_size mem) eqn:Hindex => //.
+  rewrite get_set_other => //.
+  unfold Uint63_of_N.
+  move => Hinjeq.
+  unfold vector_length in Hif.
+  move/N.ltb_spec0 in Hindex.
+  specialize (@vector_size_bound _ mem) as Hsizebound.
+  assert (i < byte_limit) as Hiub; first by lias.
+  assert (j < byte_limit) as Hjub; first by lias.
+  apply (f_equal to_Z) in Hinjeq.
+  do 2 (rewrite of_Z_spec in Hinjeq).
+  cbn in *.
+  do 2 (rewrite Z.mod_small in Hinjeq => //; last by lias).
+  by lias.
+Qed.
   
 Lemma mv_grow_length :
   forall n mem mem',
-    mv_grow n mem = mem' ->
+    mv_grow n mem = Some mem' ->
     mv_length mem' = (mv_length mem + n)%N.
 Proof.
-  move => n mem mem' Hgrow.
-  unfold mv_grow in Hgrow; subst.
-  unfold mv_length => /=.
-  admit.
-Admitted.
-
+  move => n mem mem'.
+  unfold mv_grow, vector_grow.
+  generalize (Logic.eq_refl ((vector_length mem + n) <=? byte_limit)).
+  generalize ((vector_length mem + n) <=? byte_limit) at 2 3.
+  case => Hub => //=.
+  generalize (Logic.eq_refl ((vector_length mem + n) <=? v_capacity mem)).
+  generalize ((vector_length mem + n) <=? v_capacity mem) at 2 3.
+  case => Hgrow //=; move => [<-] => /=; done.
+Qed.
+  
 Lemma mv_grow_lookup :
   forall i n mem mem',
     (i < mv_length mem)%N ->
-    mv_grow n mem = mem' ->
+    mv_grow n mem = Some mem' ->
     mv_lookup i mem' = mv_lookup i mem.
 Proof.
-  move => i n mem mem' Hlen Hgrow.
-  unfold mv_lookup.
+  move => i n mem mem' Hlen.
+  assert (i < mv_length mem + n) as Hlengrow; first by lias.
   move/N.ltb_spec0 in Hlen.
-Admitted.
+  move/N.ltb_spec0 in Hlengrow.
+  unfold mv_grow, vector_grow.
+  generalize (Logic.eq_refl ((vector_length mem + n) <=? byte_limit)).
+  generalize ((vector_length mem + n) <=? byte_limit) at 2 3.
+  case => Hub => //=.
+  generalize (Logic.eq_refl ((vector_length mem + n) <=? v_capacity mem)).
+  generalize ((vector_length mem + n) <=? v_capacity mem) at 2 3.
+  case => Hgrow //=; move => [<-] => /=; unfold mv_lookup, vector_lookup => /=; rewrite Hlen Hlengrow.
+  - done.
+  - move/N.leb_spec0 in Hub.
+    move/N.leb_spec0 in Hgrow.
+    unfold mv_length in *.
+    move/N.ltb_spec0 in Hlen.
+    move/N.ltb_spec0 in Hlengrow.
+    assert (i < byte_limit) as Hibound; first by lias.
+    specialize (@v_size_valid _ mem) as Hsize.
+    specialize (v_capacity_eq mem) as Hcap.
+    unfold Uint63_to_N in Hcap.
+    rewrite Hcap in Hsize.
+    apply Znat.N2Z.inj_le in Hsize.
+    specialize (to_Z_bounded (arr_length (v_data mem))) as HZbound.
+    rewrite Znat.Z2N.id in Hsize => //; last by lias.
+    rewrite get_make_copy => //; unfold Uint63_of_N.
+    + apply/Uint63.ltbP.
+      repeat rewrite of_Z_spec.
+      do 2 (rewrite Z.mod_small; last by cbn; cbn in Hub; lias).
+      by lias.
+    + apply/Uint63.lebP.
+      rewrite of_Z_spec.
+      rewrite Z.mod_small; by lias.
+    + apply/Uint63.ltbP.
+      rewrite of_Z_spec.
+      rewrite Z.mod_small; last by cbn; cbn in Hibound; lias.
+      unfold vector_length in Hlen.
+      by lias.
+Qed.
   
 #[export]
   Instance Memory_vec: Memory.
 Proof.
   apply (@Build_Memory memory_vec mv_make mv_length mv_lookup mv_grow mv_update).
-  - exact mv_eq_dec.
   - exact mv_lookup_oob.
   - exact mv_make_length.
   - exact mv_make_lookup.
@@ -290,51 +407,3 @@ Proof.
 Qed.
 
 End MemoryVec.
-
-(*
-
-  (*
-  (* Efficient tree building, starting from 1 *)
-Fixpoint gmap_iota (offset: positive) (len: positive) (b: byte) : gmap positive byte :=
-  match len with
-  | xH => {[ offset := b ]}
-  | xO p => (gmap_iota offset p b) ∪ (gmap_iota (offset + p) p b)
-  | xI p => <[ (offset + (xO p)) := b ]> ((gmap_iota offset p b) ∪ (gmap_iota (offset + p) p b))
-  end.
-
-(*
-Lemma gmap_iota_disjoint :
-  forall offset len b,
-    map_disjoint (gmap_iota offset len b) (gmap_iota (offset + len) len b).
-Proof.
-  move => offset len; move: offset.
-  induction len.
-Qed.
-*)
-
-Lemma gmap_iota_spec: forall offset len b,
-    map_to_list (gmap_iota offset len b) ≡
-      (List.map (fun i => (Pos.of_nat i, b)) (iota (Pos.to_nat offset) (Pos.to_nat len))).
-Proof.
-  move => offset len; move: offset.
-  induction len; move => offset b => /=.
-  (* xI *)
-  - rewrite (map_to_list_insert _ (offset+len~0) b).
-Qed.
-
-Definition mt_make : byte -> N -> memory_tree.
-Proof.
-  refine (fun v (len: N) =>
-    {| mt_init := v;
-      mt_data :=
-        match len with
-        | N0 => ∅
-        | Npos p => gmap_iota 1 p v
-        end;
-      mt_size := len
-    |}).
-  
-Defined.
-*)
-End MemoryList.
-*)
